<?xml version="1.0" encoding="UTF-8"?>
<section xml:id="sec-6_3">
  <title>Delta Functions and Forcing</title>

  <exercises xml:id="exercises-6_3">
    <exercisegroup xml:id="exercisegroup-Supplemental_HW_Problems-6_3">
      <title>Supplemental HW Problems</title>
      <introduction>
        <p>
          The Dirac Delta function is defined as a <q>quick</q> impact, so that at a time <m>t = t_0</m> we have an impulse of magnitude <m>1,</m> but zero everywhere else.
        </p>
        <p>
          In other words: <m>\delta(t-t_0)=0</m> for <m>t\neq t_0</m> but
          <me>\int_{-\infty}^\infty\delta(t-t_0)dt=1</me>
          We can break the above integral up:
          <me>\int_{-\infty}^\infty\delta(t-t_0)=\int_{-\infty}^c\delta(t-t_0)+\int_c^\infty\delta(t-t_0)</me>
        </p>
      </introduction>
      <exercise>
        <statement>
          <p>
            From the right side of the equation above, consider the integral <me>\int_{-\infty}^c\delta(t-t_0)</me>
            What is the value of this integral when <m>c \lt t_0?</m>  What is the value of this integral when <m>c \gt t_0?</m>  Write the single integral above as a piecewise function in that way.
          </p>
        </statement>
        <answer>
          <p>
            <m>k(x)=f(x)+6</m>. So, we can shift the graph of <m>y=f(x)</m> up <m>6</m> units to obtain <m>y=k(x)</m>.
          </p>
        </answer>
      </exercise>
      <exercise>
        <statement>
          <p>
            The Heaviside function is defined as:
            <me>u_c(t) = \begin{cases} 0 \amp \text{if } t \lt c \\
           1 \amp \text{if } t \geq c \end{cases}</me>
            What does that tell us about the integral in problem 1 and the Heaviside function?
          </p>
        </statement>
        <answer>
          <p>
            <m>k(x)=f(x)+6</m>. So, we can shift the graph of <m>y=f(x)</m> up <m>6</m> units to obtain <m>y=k(x)</m>.
          </p>
        </answer>
      </exercise>
      <exercise>
        <statement>
          <p>
            Since the Heaviside function and the integral we found in problem 1 are the same, take a derivative of both sides.  What does that mean as far as the relationship between the Heaviside function and the Dirac Delta function?
          </p>
        </statement>
        <answer>
          <p>
            <m>k(x)=f(x)+6</m>. So, we can shift the graph of <m>y=f(x)</m> up <m>6</m> units to obtain <m>y=k(x)</m>.
          </p>
        </answer>
      </exercise>
      <exercise>
        <statement>
          <p>
            A spring-mass system involves a mass of <m>1</m> kg, an external friction coefficient of <m>2</m> kg/sec, and a spring constant of <m>10</m> kg/s<m>^2.</m>  At time <m>t = 0,</m> the spring is stretched out by <m>2</m> meters from rest and released.  At <m>t = 5,</m> a hammer smashes into the mass with a force of <m>2</m> Newtons.
          </p>
          <ol>
            <li><p>What do you expect to happen here?  Talk about short-run behavior and events, and the long-term behavior of this system.</p></li>
            <li><p>Pick the best equation for the position of the mass from the choices below:</p>
              <ol>
                <li><p><me>x'' + 2x’ + 10x = 2u_0(t)</me></p></li>
                <li><p><me>x'' + 2x’ + 10x = 2u_5(t)</me></p></li>
                <li><p><me>x'' + 2x’ + 10x = 2u(t-5)</me></p></li>
                <li><p><me>x'' + 2x’ + 10x = 2\delta(t)</me></p></li>
                <li><p><me>x'' + 2x’ + 10x = 2\delta(5)</me></p></li>
                <li><p><me>x'' + 2x’ + 10x = 2\delta(t-5)</me></p></li>
              </ol>
            </li>
            <li><p>Using Laplace transforms, find <m>x(t)</m>.</p></li>
            <li><p>Does your function match up with what you expected from part (a) – does the function for <m>x(t)</m> match the situation, in the short-run and long-term?</p></li>
          </ol>
        </statement>
        <answer>
          <p>
            <m>k(x)=f(x)+6</m>. So, we can shift the graph of <m>y=f(x)</m> up <m>6</m> units to obtain <m>y=k(x)</m>.
          </p>
        </answer>
      </exercise>
    </exercisegroup>

    <exercisegroup xml:id="exercisegroup-Appendix_to-6_3">
      <title>Appendix to Judson's 6.3</title>
      <introduction>
        <p>
          One of the examples in the text refers to <m>\sinh</m> and <m>\cosh.</m>  These are the Hyperbolic Functions, and we pronounce <m>\sinh</m> as <q>sinch</q> and <m>\cosh</m> as <q>cosh.</q>  They are, put very roughly, a way to do periodic function work with exponential functions because of the way they are defined:
        </p>
        <p><md>
          <mrow>\sinh(x) \amp = \frac{e^x-e^{-x}}{2}</mrow>
          <mrow>\cosh(x) \amp = \frac{e^x+e^{-x}}{2}</mrow>
        </md></p>
        <p>
          The derivative of <m>\sinh</m> is <m>\cosh,</m> and the derivative of <m>\cosh</m> is <m>\sinh</m>.
        </p>
      </introduction>
      <exercise>
        <statement>
          <p>
            Take derivatives of both to verify this!
          </p>
          <p>
            We have a variety of trig-like identities with these objects, and you can find a summary of these (and more information) at the <url href="https://en.wikipedia.org/wiki/Hyperbolic_functions">Wikipedia page</url>. A few of the important ones are:
          </p>
          <p><md>
            <mrow>\sinh(-x) \amp = -\sinh(x)</mrow>
            <mrow>\cosh(-x) \amp = \cosh(x)</mrow>
            <mrow>\cosh(x) + \sinh(x) \amp = e^x</mrow>
            <mrow>\cosh(x) - \sinh(x) \amp = e^{-x}</mrow>
            <mrow>\cosh^2(x) - \sinh^2(x) \amp = 1</mrow>
          </md></p>
        </statement>
        <answer>
          <p>
            <m>g(x)=f(-x)</m>. So, we can reflect the graph of <m>y=f(x)</m> across the <m>y</m>-axis to obtain <m>y=g(x)</m>.
          </p>
        </answer>
      </exercise>
      <exercise>
        <statement>
          <p>
            Show these algebraically!
          </p>
          <p>
            And an interesting analysis of these can be found <url href="https://www.math.purdue.edu/~pvankoug/math266/sinh_cosh_sin_cos.pdf">on this website</url> from Purdue University.
          </p>
        </statement>
        <answer>
          <p>
            <m>g(x)=f(-x)</m>. So, we can reflect the graph of <m>y=f(x)</m> across the <m>y</m>-axis to obtain <m>y=g(x)</m>.
          </p>
        </answer>
      </exercise>
    </exercisegroup>

  </exercises>

</section>
